proof/amd64/extracted/Keccak1600_Jazz.ec
@@ -7,7 +7,12 @@ import SLH64.
 require import
 Array1 Array3 Array5 Array6 Array7 Array24 Array25 Array26 Array101 WArray3
 WArray32 WArray40 WArray160 WArray192 WArray200 WArray208 WArray224 WArray800
-WArray808.
+WArray808 ArrayWords25W64 ArrayWords26W64 ArrayWords101W64 ArrayWords25W256
+SubArray25_26 SubArrayDirect25W256_101W64 ArrayAccessCastW8_25W64
+ArrayAccessCastW8_26W64 ArrayAccessCastW8_101W64 ArrayAccessCastW32_26W64
+ArrayAccessCastW32_101W64 ArrayAccessCastW64_25W64 ArrayAccessCastW64_25W256
+ArrayAccessCastW256_25W64 ArrayAccessCastW256_26W64
+ArrayAccessCastW256_101W64 ArrayAccessCastW256_25W256.
 
 abbrev rOL8 =
 ((Array1.of_list witness)
@@ -264,11 +269,9 @@ module M = {
   proc __addratebit_ref (st:W64.t Array25.t, _RATE8:int) : W64.t Array25.t = {
     
     st <-
-    (Array25.init
-    (WArray200.get64
-    (WArray200.set8_direct (WArray200.init64 (fun i => st.[i])) (_RATE8 - 1)
-    ((get8_direct (WArray200.init64 (fun i => st.[i])) (_RATE8 - 1)) `^`
-    (W8.of_int 128)))));
+    (ArrayAccessCastW8_25W64.set_cast_direct st (_RATE8 - 1)
+    ((ArrayAccessCastW8_25W64.get_cast_direct st (_RATE8 - 1)) `^`
+    (W8.of_int 128)));
     return st;
   }
   proc __SHLQ (x:W64.t, shbytes:int) : W64.t = {
@@ -1511,27 +1514,21 @@ module M = {
     var t256_2:W256.t;
     state <- witness;
     state.[0] <-
-    (VPBROADCAST_4u64
-    (get64_direct (WArray200.init64 (fun i => st.[i])) (8 * 0)));
-    state.[1] <-
-    (get256_direct (WArray200.init64 (fun i => st.[i])) (1 * 8));
+    (VPBROADCAST_4u64 (ArrayAccessCastW64_25W64.get_cast_direct st (8 * 0)));
+    state.[1] <- (ArrayAccessCastW256_25W64.get_cast_direct st (1 * 8));
     t128_1 <- (VMOV_64 st.[5]);
-    state.[3] <-
-    (get256_direct (WArray200.init64 (fun i => st.[i])) (6 * 8));
+    state.[3] <- (ArrayAccessCastW256_25W64.get_cast_direct st (6 * 8));
     t128_0 <- (VMOV_64 st.[10]);
-    state.[4] <-
-    (get256_direct (WArray200.init64 (fun i => st.[i])) (11 * 8));
+    state.[4] <- (ArrayAccessCastW256_25W64.get_cast_direct st (11 * 8));
     r <- st.[15];
     t128_1 <- (VPINSR_2u64 t128_1 r (W8.of_int 1));
-    state.[5] <-
-    (get256_direct (WArray200.init64 (fun i => st.[i])) (16 * 8));
+    state.[5] <- (ArrayAccessCastW256_25W64.get_cast_direct st (16 * 8));
     r <- st.[20];
     t128_0 <- (VPINSR_2u64 t128_0 r (W8.of_int 1));
     t256_0 <- (zeroextu256 t128_0);
     t256_0 <- (VINSERTI128 t256_0 t128_1 (W8.of_int 1));
     state.[2] <- t256_0;
-    state.[6] <-
-    (get256_direct (WArray200.init64 (fun i => st.[i])) (21 * 8));
+    state.[6] <- (ArrayAccessCastW256_25W64.get_cast_direct st (21 * 8));
     t256_0 <-
     (VPBLEND_8u32 state.[3] state.[5]
     (W8.of_int
@@ -1665,11 +1662,7 @@ module M = {
     var t256_4:W256.t;
     t128_0 <- (truncateu128 state.[0]);
     st.[0] <- (VMOVLPD t128_0);
-    st <-
-    (Array25.init
-    (WArray200.get64
-    (WArray200.set256_direct (WArray200.init64 (fun i => st.[i])) (1 * 8)
-    state.[1])));
+    st <- (ArrayAccessCastW256_25W64.set_cast_direct st (1 * 8) state.[1]);
     t256_0 <-
     (VPBLEND_8u32 state.[3] state.[4]
     (W8.of_int
@@ -1747,11 +1740,7 @@ module M = {
     ((2 ^ 1) *
     ((0 %% (2 ^ 1)) + ((2 ^ 1) * ((1 %% (2 ^ 1)) + ((2 ^ 1) * 1))))))))))))))
     ));
-    st <-
-    (Array25.init
-    (WArray200.get64
-    (WArray200.set256_direct (WArray200.init64 (fun i => st.[i])) (6 * 8)
-    t256_4)));
+    st <- (ArrayAccessCastW256_25W64.set_cast_direct st (6 * 8) t256_4);
     t128_0 <- (truncateu128 state.[2]);
     st.[10] <- (VMOVLPD t128_0);
     t256_4 <-
@@ -1769,11 +1758,7 @@ module M = {
     ((2 ^ 1) *
     ((0 %% (2 ^ 1)) + ((2 ^ 1) * ((1 %% (2 ^ 1)) + ((2 ^ 1) * 1))))))))))))))
     ));
-    st <-
-    (Array25.init
-    (WArray200.get64
-    (WArray200.set256_direct (WArray200.init64 (fun i => st.[i])) (11 * 8)
-    t256_4)));
+    st <- (ArrayAccessCastW256_25W64.set_cast_direct st (11 * 8) t256_4);
     st.[15] <- (VMOVHPD t128_1);
     t256_4 <-
     (VPBLEND_8u32 t256_2 t256_0
@@ -1790,11 +1775,7 @@ module M = {
     ((2 ^ 1) *
     ((0 %% (2 ^ 1)) + ((2 ^ 1) * ((1 %% (2 ^ 1)) + ((2 ^ 1) * 1))))))))))))))
     ));
-    st <-
-    (Array25.init
-    (WArray200.get64
-    (WArray200.set256_direct (WArray200.init64 (fun i => st.[i])) (16 * 8)
-    t256_4)));
+    st <- (ArrayAccessCastW256_25W64.set_cast_direct st (16 * 8) t256_4);
     st.[20] <- (VMOVHPD t128_0);
     t256_4 <-
     (VPBLEND_8u32 t256_1 t256_2
@@ -1811,11 +1792,7 @@ module M = {
     ((2 ^ 1) *
     ((0 %% (2 ^ 1)) + ((2 ^ 1) * ((1 %% (2 ^ 1)) + ((2 ^ 1) * 1))))))))))))))
     ));
-    st <-
-    (Array25.init
-    (WArray200.get64
-    (WArray200.set256_direct (WArray200.init64 (fun i => st.[i])) (21 * 8)
-    t256_4)));
+    st <- (ArrayAccessCastW256_25W64.set_cast_direct st (21 * 8) t256_4);
     return st;
   }
   proc _keccakf1600_st25_avx2 (st25:W64.t Array25.t) : W64.t Array25.t = {
@@ -2572,10 +2549,7 @@ module M = {
     r256 <- (set0_256);
     i <- 0;
     while ((i < 6)) {
-      st <-
-      (Array26.init
-      (WArray208.get64
-      (WArray208.set256 (WArray208.init64 (fun i_0 => st.[i_0])) i r256)));
+      st <- (ArrayAccessCastW256_26W64.set_cast st i r256);
       i <- (i + 1);
     }
     st.[24] <- (W64.of_int 0);
@@ -2621,22 +2595,16 @@ module M = {
     ststatus <- st.[25];
     (trailb, r8, at) <@ _ststatus_data (ststatus);
     st <-
-    (Array26.init
-    (WArray208.get64
-    (WArray208.set8_direct (WArray208.init64 (fun i => st.[i])) at
-    ((get8_direct (WArray208.init64 (fun i => st.[i])) at) `^` trailb))));
+    (ArrayAccessCastW8_26W64.set_cast_direct st at
+    ((ArrayAccessCastW8_26W64.get_cast_direct st at) `^` trailb));
     st <-
-    (Array26.init
-    (WArray208.get64
-    (WArray208.set8_direct (WArray208.init64 (fun i => st.[i])) (r8 - 1)
-    ((get8_direct (WArray208.init64 (fun i => st.[i])) (r8 - 1)) `^`
-    (W8.of_int 128)))));
+    (ArrayAccessCastW8_26W64.set_cast_direct st (r8 - 1)
+    ((ArrayAccessCastW8_26W64.get_cast_direct st (r8 - 1)) `^`
+    (W8.of_int 128)));
     st <-
-    (Array26.init
-    (WArray208.get64
-    (WArray208.set32_direct (WArray208.init64 (fun i => st.[i])) (8 * 25)
-    ((get32_direct (WArray208.init64 (fun i => st.[i])) (8 * 25)) `&`
-    (W32.of_int 4278255360)))));
+    (ArrayAccessCastW32_26W64.set_cast_direct st (8 * 25)
+    ((ArrayAccessCastW32_26W64.get_cast_direct st (8 * 25)) `&`
+    (W32.of_int 4278255360)));
     return st;
   }
   proc keccak_ststatus (status:W8.t Array3.t, st:W64.t Array26.t) : W8.t Array3.t = {
@@ -2649,7 +2617,7 @@ module M = {
     status.[0] <- (truncateu8 (W64.of_int r8));
     status.[1] <- (truncateu8 (W64.of_int at));
     status.[2] <-
-    (get8_direct (WArray208.init64 (fun i => st.[i])) ((8 * 25) + 2));
+    (ArrayAccessCastW8_26W64.get_cast_direct st ((8 * 25) + 2));
     return status;
   }
   proc init_updstate_avx2 (st:W64.t Array26.t, r64:int, trailb:W8.t) : 
@@ -2689,10 +2657,8 @@ module M = {
       sh <- (sh `<<` (W8.of_int 3));
       t64 <- (t64 `<<` (sh `&` (W8.of_int 63)));
       st <-
-      (Array25.init
-      (WArray200.get64
-      (WArray200.set64_direct (WArray200.init64 (fun i => st.[i])) at
-      ((get64_direct (WArray200.init64 (fun i => st.[i])) at) `^` t64))));
+      (ArrayAccessCastW64_25W64.set_cast_direct st at
+      ((ArrayAccessCastW64_25W64.get_cast_direct st at) `^` t64));
       if ((8 <= len)) {
         buf <- (buf + 8);
         buf <- (buf - (W64.to_uint at8));
@@ -2709,10 +2675,8 @@ module M = {
     while ((newat <= upto)) {
       t64 <- (loadW64 Glob.mem buf);
       st <-
-      (Array25.init
-      (WArray200.get64
-      (WArray200.set64_direct (WArray200.init64 (fun i => st.[i])) at
-      ((get64_direct (WArray200.init64 (fun i => st.[i])) at) `^` t64))));
+      (ArrayAccessCastW64_25W64.set_cast_direct st at
+      ((ArrayAccessCastW64_25W64.get_cast_direct st at) `^` t64));
       at <- newat;
       buf <- (buf + 8);
       newat <- (newat + 8);
@@ -2722,10 +2686,8 @@ module M = {
       upto8 <- (upto8 `&` (W64.of_int 7));
       (buf, t64) <@ __m_rlen_read_upto8 (buf, (W64.to_uint upto8));
       st <-
-      (Array25.init
-      (WArray200.get64
-      (WArray200.set64_direct (WArray200.init64 (fun i => st.[i])) at
-      ((get64_direct (WArray200.init64 (fun i => st.[i])) at) `^` t64))));
+      (ArrayAccessCastW64_25W64.set_cast_direct st at
+      ((ArrayAccessCastW64_25W64.get_cast_direct st at) `^` t64));
     } else {
       
     }
@@ -2743,7 +2705,7 @@ module M = {
     stk <- witness;
     ststatus <- st.[25];
     ( _0, r8, at) <@ _ststatus_data (ststatus);
-    stk <- (Array25.init (fun i => st.[(0 + i)]));
+    stk <- (SubArray25_26.get_sub st 0);
     (* Erased call to spill *)
     len <- (len + at);
     while ((r8 <= len)) {
@@ -2755,14 +2717,10 @@ module M = {
     len <- len;
     (* Erased call to unspill *)
     (stk, at,  _1) <@ _add_m_updstate_avx2 (stk, at, buf, len);
+    st <- (SubArray25_26.set_sub st 0 stk);
     st <-
-    (Array26.init
-    (fun i => (if (0 <= i < (0 + 25)) then stk.[(i - 0)] else st.[i])));
-    st <-
-    (Array26.init
-    (WArray208.get64
-    (WArray208.set8_direct (WArray208.init64 (fun i => st.[i])) (8 * 25)
-    (truncateu8 (W64.of_int at)))));
+    (ArrayAccessCastW8_26W64.set_cast_direct st (8 * 25)
+    (truncateu8 (W64.of_int at)));
     return st;
   }
   proc _dump_m_updstate_avx2 (buf:int, st:W64.t Array25.t, at:int, upto:int) : 
@@ -2781,7 +2739,7 @@ module M = {
       len <- (len - at);
       at <- (at `|>>` 3);
       at <- (at `<<` 3);
-      t64 <- (get64_direct (WArray200.init64 (fun i => st.[i])) at);
+      t64 <- (ArrayAccessCastW64_25W64.get_cast_direct st at);
       sh <- (truncateu8 at8);
       sh <- (sh `<<` (W8.of_int 3));
       t64 <- (t64 `>>` (sh `&` (W8.of_int 63)));
@@ -2801,7 +2759,7 @@ module M = {
     newat <- at;
     newat <- (newat + 8);
     while ((newat <= upto)) {
-      t64 <- (get64_direct (WArray200.init64 (fun i => st.[i])) at);
+      t64 <- (ArrayAccessCastW64_25W64.get_cast_direct st at);
       Glob.mem <- (storeW64 Glob.mem buf t64);
       at <- newat;
       buf <- (buf + 8);
@@ -2810,7 +2768,7 @@ module M = {
     if ((at < upto)) {
       upto8 <- (W64.of_int upto);
       upto8 <- (upto8 `&` (W64.of_int 7));
-      t64 <- (get64_direct (WArray200.init64 (fun i => st.[i])) at);
+      t64 <- (ArrayAccessCastW64_25W64.get_cast_direct st at);
       buf <@ __m_rlen_write_upto8 (buf, t64, (W64.to_uint upto8));
     } else {
       
@@ -2828,7 +2786,7 @@ module M = {
     stk <- witness;
     ststatus <- st.[25];
     ( _0, r8, at) <@ _ststatus_data (ststatus);
-    stk <- (Array25.init (fun i => st.[(0 + i)]));
+    stk <- (SubArray25_26.get_sub st 0);
     (* Erased call to spill *)
     if ((at = 0)) {
       stk <@ _keccakf1600_st25_avx2 (stk);
@@ -2848,14 +2806,10 @@ module M = {
     len <- len;
     (buf, at) <@ _dump_m_updstate_avx2 (buf, stk, at, len);
     (* Erased call to unspill *)
+    st <- (SubArray25_26.set_sub st 0 stk);
     st <-
-    (Array26.init
-    (fun i => (if (0 <= i < (0 + 25)) then stk.[(i - 0)] else st.[i])));
-    st <-
-    (Array26.init
-    (WArray208.get64
-    (WArray208.set8_direct (WArray208.init64 (fun i => st.[i])) (8 * 25)
-    (truncateu8 (W64.of_int at)))));
+    (ArrayAccessCastW8_26W64.set_cast_direct st (8 * 25)
+    (truncateu8 (W64.of_int at)));
     return (buf, st);
   }
   proc absorb_m_updstate_avx2 (st:W64.t Array26.t, buf:int, len:int) : 
@@ -2904,10 +2858,10 @@ module M = {
     var t3:W64.t;
     i <- 0;
     while ((i < 6)) {
-      x0 <- (get256 (WArray200.init64 (fun i_0 => st0.[i_0])) i);
-      x1 <- (get256 (WArray200.init64 (fun i_0 => st1.[i_0])) i);
-      x2 <- (get256 (WArray200.init64 (fun i_0 => st2.[i_0])) i);
-      x3 <- (get256 (WArray200.init64 (fun i_0 => st3.[i_0])) i);
+      x0 <- (ArrayAccessCastW256_25W64.get_cast st0 i);
+      x1 <- (ArrayAccessCastW256_25W64.get_cast st1 i);
+      x2 <- (ArrayAccessCastW256_25W64.get_cast st2 i);
+      x3 <- (ArrayAccessCastW256_25W64.get_cast st3 i);
       (x0, x1, x2, x3) <@ __u256x4_4u64x4 (x0, x1, x2, x3);
       st4x.[((4 * i) + 0)] <- x0;
       st4x.[((4 * i) + 1)] <- x1;
@@ -2919,26 +2873,10 @@ module M = {
     t1 <- st1.[24];
     t2 <- st2.[24];
     t3 <- st3.[24];
-    st4x <-
-    (Array25.init
-    (WArray800.get256
-    (WArray800.set64 (WArray800.init256 (fun i_0 => st4x.[i_0]))
-    ((4 * 24) + 0) t0)));
-    st4x <-
-    (Array25.init
-    (WArray800.get256
-    (WArray800.set64 (WArray800.init256 (fun i_0 => st4x.[i_0]))
-    ((4 * 24) + 1) t1)));
-    st4x <-
-    (Array25.init
-    (WArray800.get256
-    (WArray800.set64 (WArray800.init256 (fun i_0 => st4x.[i_0]))
-    ((4 * 24) + 2) t2)));
-    st4x <-
-    (Array25.init
-    (WArray800.get256
-    (WArray800.set64 (WArray800.init256 (fun i_0 => st4x.[i_0]))
-    ((4 * 24) + 3) t3)));
+    st4x <- (ArrayAccessCastW64_25W256.set_cast st4x ((4 * 24) + 0) t0);
+    st4x <- (ArrayAccessCastW64_25W256.set_cast st4x ((4 * 24) + 1) t1);
+    st4x <- (ArrayAccessCastW64_25W256.set_cast st4x ((4 * 24) + 2) t2);
+    st4x <- (ArrayAccessCastW64_25W256.set_cast st4x ((4 * 24) + 3) t3);
     return st4x;
   }
   proc __4u64x4_u256x4 (y0:W256.t, y1:W256.t, y2:W256.t, y3:W256.t) : 
@@ -2980,31 +2918,19 @@ module M = {
       x3 <- st4x.[((4 * i) + 3)];
       (x0, x1, x2, x3) <@ __4u64x4_u256x4 (x0, x1, x2, x3);
       st0 <-
-      (Array25.init
-      (WArray200.get64
-      (WArray200.set256_direct (WArray200.init64 (fun i_0 => st0.[i_0]))
-      ((4 * 8) * i) x0)));
+      (ArrayAccessCastW256_25W64.set_cast_direct st0 ((4 * 8) * i) x0);
       st1 <-
-      (Array25.init
-      (WArray200.get64
-      (WArray200.set256_direct (WArray200.init64 (fun i_0 => st1.[i_0]))
-      ((4 * 8) * i) x1)));
+      (ArrayAccessCastW256_25W64.set_cast_direct st1 ((4 * 8) * i) x1);
       st2 <-
-      (Array25.init
-      (WArray200.get64
-      (WArray200.set256_direct (WArray200.init64 (fun i_0 => st2.[i_0]))
-      ((4 * 8) * i) x2)));
+      (ArrayAccessCastW256_25W64.set_cast_direct st2 ((4 * 8) * i) x2);
       st3 <-
-      (Array25.init
-      (WArray200.get64
-      (WArray200.set256_direct (WArray200.init64 (fun i_0 => st3.[i_0]))
-      ((4 * 8) * i) x3)));
+      (ArrayAccessCastW256_25W64.set_cast_direct st3 ((4 * 8) * i) x3);
       i <- (i + 1);
     }
-    t0 <- (get64 (WArray800.init256 (fun i_0 => st4x.[i_0])) ((4 * 24) + 0));
-    t1 <- (get64 (WArray800.init256 (fun i_0 => st4x.[i_0])) ((4 * 24) + 1));
-    t2 <- (get64 (WArray800.init256 (fun i_0 => st4x.[i_0])) ((4 * 24) + 2));
-    t3 <- (get64 (WArray800.init256 (fun i_0 => st4x.[i_0])) ((4 * 24) + 3));
+    t0 <- (ArrayAccessCastW64_25W256.get_cast st4x ((4 * 24) + 0));
+    t1 <- (ArrayAccessCastW64_25W256.get_cast st4x ((4 * 24) + 1));
+    t2 <- (ArrayAccessCastW64_25W256.get_cast st4x ((4 * 24) + 2));
+    t3 <- (ArrayAccessCastW64_25W256.get_cast st4x ((4 * 24) + 3));
     st0.[24] <- t0;
     st1.[24] <- t1;
     st2.[24] <- t2;
@@ -4753,32 +4679,6 @@ module M = {
     st.[24] <- y2;
     return st;
   }
-  proc test_keccakf1600x4_native (st:W256.t Array25.t, c:W64.t) : W256.t Array25.t = {
-    var y10:W256.t;
-    var y14:W256.t;
-    var y8:W256.t;
-    var y15:W256.t;
-    var y9:W256.t;
-    var y13:W256.t;
-    var y3:W256.t;
-    var y7:W256.t;
-    var y2:W256.t;
-    var rol8:W256.t Array1.t;
-    var rol56:W256.t Array1.t;
-    var rc:W64.t Array24.t;
-    rc <- witness;
-    rol56 <- witness;
-    rol8 <- witness;
-    (y10, y14, y8, y15, y9, y13, y3, y7, y2) <@ __regs_fetch (st);
-    rol8 <- rOL8;
-    rol56 <- rOL56;
-    rc <- kECCAK1600_RC;
-    (st, y10, y14, y8, y15, y9, y13, y3, y7, y2) <@ __f1600_loopbody_native (
-    st, rol8, rol56, rc, (W64.to_uint c), y10, y14, y8, y15, y9, y13, 
-    y3, y7, y2);
-    st <@ __regs_unfetch (st, y10, y14, y8, y15, y9, y13, y3, y7, y2);
-    return st;
-  }
   proc __keccakf1600_avx2x4_native (st:W256.t Array25.t) : W256.t Array25.t = {
     var y10:W256.t;
     var y14:W256.t;
@@ -4835,11 +4735,7 @@ module M = {
     z256 <- (set0_256);
     i <- 0;
     while ((i < (32 * 25))) {
-      st <-
-      (Array25.init
-      (WArray800.get256
-      (WArray800.set256_direct (WArray800.init256 (fun i_0 => st.[i_0])) 
-      i z256)));
+      st <- (ArrayAccessCastW256_25W256.set_cast_direct st i z256);
       i <- (i + 32);
     }
     return st;
@@ -4877,11 +4773,8 @@ module M = {
     while ((at < (32 * ((aT %/ 8) + (_LEN %/ 8))))) {
       w <- (VPBROADCAST_4u64 (loadW64 Glob.mem buf));
       buf <- (buf + 8);
-      w <- (w `^` (get256_direct (WArray800.init256 (fun i => st.[i])) at));
-      st <-
-      (Array25.init
-      (WArray800.get256
-      (WArray800.set256_direct (WArray800.init256 (fun i => st.[i])) at w)));
+      w <- (w `^` (ArrayAccessCastW256_25W256.get_cast_direct st at));
+      st <- (ArrayAccessCastW256_25W256.set_cast_direct st at w);
       at <- (at + 32);
     }
     aT <- (aT + (8 * (_LEN %/ 8)));
@@ -4889,11 +4782,8 @@ module M = {
     if (((0 < _LEN) \/ ((_TRAILB %% 256) <> 0))) {
       (buf, _LEN, _TRAILB, aT, w) <@ __m_ilen_read_bcast_upto8_at (buf, 
       _LEN, _TRAILB, aT, aT);
-      w <- (w `^` (get256_direct (WArray800.init256 (fun i => st.[i])) at));
-      st <-
-      (Array25.init
-      (WArray800.get256
-      (WArray800.set256_direct (WArray800.init256 (fun i => st.[i])) at w)));
+      w <- (w `^` (ArrayAccessCastW256_25W256.get_cast_direct st at));
+      st <- (ArrayAccessCastW256_25W256.set_cast_direct st at w);
     } else {
       
     }
@@ -4965,39 +4855,23 @@ module M = {
       (buf0,  _0,  _1,  _2, t0) <@ __m_ilen_read_upto8_at (buf0, _LEN,
       _TRAILB, aT, aT8);
       st <-
-      (Array25.init
-      (WArray800.get256
-      (WArray800.set64 (WArray800.init256 (fun i => st.[i]))
-      ((4 * (aT %/ 8)) + 0)
-      ((get64 (WArray800.init256 (fun i => st.[i])) ((4 * (aT %/ 8)) + 0)) `^`
-      t0))));
+      (ArrayAccessCastW64_25W256.set_cast st ((4 * (aT %/ 8)) + 0)
+      ((ArrayAccessCastW64_25W256.get_cast st ((4 * (aT %/ 8)) + 0)) `^` t0));
       (buf1,  _3,  _4,  _5, t1) <@ __m_ilen_read_upto8_at (buf1, _LEN,
       _TRAILB, aT, aT8);
       st <-
-      (Array25.init
-      (WArray800.get256
-      (WArray800.set64 (WArray800.init256 (fun i => st.[i]))
-      ((4 * (aT %/ 8)) + 1)
-      ((get64 (WArray800.init256 (fun i => st.[i])) ((4 * (aT %/ 8)) + 1)) `^`
-      t1))));
+      (ArrayAccessCastW64_25W256.set_cast st ((4 * (aT %/ 8)) + 1)
+      ((ArrayAccessCastW64_25W256.get_cast st ((4 * (aT %/ 8)) + 1)) `^` t1));
       (buf2,  _6,  _7,  _8, t2) <@ __m_ilen_read_upto8_at (buf2, _LEN,
       _TRAILB, aT, aT8);
       st <-
-      (Array25.init
-      (WArray800.get256
-      (WArray800.set64 (WArray800.init256 (fun i => st.[i]))
-      ((4 * (aT %/ 8)) + 2)
-      ((get64 (WArray800.init256 (fun i => st.[i])) ((4 * (aT %/ 8)) + 2)) `^`
-      t2))));
+      (ArrayAccessCastW64_25W256.set_cast st ((4 * (aT %/ 8)) + 2)
+      ((ArrayAccessCastW64_25W256.get_cast st ((4 * (aT %/ 8)) + 2)) `^` t2));
       (buf3, _LEN, _TRAILB, aT8, t3) <@ __m_ilen_read_upto8_at (buf3, 
       _LEN, _TRAILB, aT, aT8);
       st <-
-      (Array25.init
-      (WArray800.get256
-      (WArray800.set64 (WArray800.init256 (fun i => st.[i]))
-      ((4 * (aT %/ 8)) + 3)
-      ((get64 (WArray800.init256 (fun i => st.[i])) ((4 * (aT %/ 8)) + 3)) `^`
-      t3))));
+      (ArrayAccessCastW64_25W256.set_cast st ((4 * (aT %/ 8)) + 3)
+      ((ArrayAccessCastW64_25W256.get_cast st ((4 * (aT %/ 8)) + 3)) `^` t3));
       aT <- aT8;
     } else {
       
@@ -5007,31 +4881,23 @@ module M = {
       t0 <- (loadW64 Glob.mem buf0);
       buf0 <- (buf0 + 8);
       st <-
-      (Array25.init
-      (WArray800.get256
-      (WArray800.set64 (WArray800.init256 (fun i => st.[i])) (at + 0)
-      ((get64 (WArray800.init256 (fun i => st.[i])) (at + 0)) `^` t0))));
+      (ArrayAccessCastW64_25W256.set_cast st (at + 0)
+      ((ArrayAccessCastW64_25W256.get_cast st (at + 0)) `^` t0));
       t1 <- (loadW64 Glob.mem buf1);
       buf1 <- (buf1 + 8);
       st <-
-      (Array25.init
-      (WArray800.get256
-      (WArray800.set64 (WArray800.init256 (fun i => st.[i])) (at + 1)
-      ((get64 (WArray800.init256 (fun i => st.[i])) (at + 1)) `^` t1))));
+      (ArrayAccessCastW64_25W256.set_cast st (at + 1)
+      ((ArrayAccessCastW64_25W256.get_cast st (at + 1)) `^` t1));
       t2 <- (loadW64 Glob.mem buf2);
       buf2 <- (buf2 + 8);
       st <-
-      (Array25.init
-      (WArray800.get256
-      (WArray800.set64 (WArray800.init256 (fun i => st.[i])) (at + 2)
-      ((get64 (WArray800.init256 (fun i => st.[i])) (at + 2)) `^` t2))));
+      (ArrayAccessCastW64_25W256.set_cast st (at + 2)
+      ((ArrayAccessCastW64_25W256.get_cast st (at + 2)) `^` t2));
       t3 <- (loadW64 Glob.mem buf3);
       buf3 <- (buf3 + 8);
       st <-
-      (Array25.init
-      (WArray800.get256
-      (WArray800.set64 (WArray800.init256 (fun i => st.[i])) (at + 3)
-      ((get64 (WArray800.init256 (fun i => st.[i])) (at + 3)) `^` t3))));
+      (ArrayAccessCastW64_25W256.set_cast st (at + 3)
+      ((ArrayAccessCastW64_25W256.get_cast st (at + 3)) `^` t3));
       at <- (at + 4);
     }
     aT <- (aT + (8 * (_LEN %/ 8)));
@@ -5040,31 +4906,23 @@ module M = {
       (buf0,  _9,  _10,  _11, t0) <@ __m_ilen_read_upto8_at (buf0, _LEN,
       _TRAILB, aT, aT);
       st <-
-      (Array25.init
-      (WArray800.get256
-      (WArray800.set64 (WArray800.init256 (fun i => st.[i])) (at + 0)
-      ((get64 (WArray800.init256 (fun i => st.[i])) (at + 0)) `^` t0))));
+      (ArrayAccessCastW64_25W256.set_cast st (at + 0)
+      ((ArrayAccessCastW64_25W256.get_cast st (at + 0)) `^` t0));
       (buf1,  _12,  _13,  _14, t1) <@ __m_ilen_read_upto8_at (buf1, _LEN,
       _TRAILB, aT, aT);
       st <-
-      (Array25.init
-      (WArray800.get256
-      (WArray800.set64 (WArray800.init256 (fun i => st.[i])) (at + 1)
-      ((get64 (WArray800.init256 (fun i => st.[i])) (at + 1)) `^` t1))));
+      (ArrayAccessCastW64_25W256.set_cast st (at + 1)
+      ((ArrayAccessCastW64_25W256.get_cast st (at + 1)) `^` t1));
       (buf2,  _15,  _16,  _17, t2) <@ __m_ilen_read_upto8_at (buf2, _LEN,
       _TRAILB, aT, aT);
       st <-
-      (Array25.init
-      (WArray800.get256
-      (WArray800.set64 (WArray800.init256 (fun i => st.[i])) (at + 2)
-      ((get64 (WArray800.init256 (fun i => st.[i])) (at + 2)) `^` t2))));
+      (ArrayAccessCastW64_25W256.set_cast st (at + 2)
+      ((ArrayAccessCastW64_25W256.get_cast st (at + 2)) `^` t2));
       (buf3,  _18,  _19, aT, t3) <@ __m_ilen_read_upto8_at (buf3, _LEN,
       _TRAILB, aT, aT);
       st <-
-      (Array25.init
-      (WArray800.get256
-      (WArray800.set64 (WArray800.init256 (fun i => st.[i])) (at + 3)
-      ((get64 (WArray800.init256 (fun i => st.[i])) (at + 3)) `^` t3))));
+      (ArrayAccessCastW64_25W256.set_cast st (at + 3)
+      ((ArrayAccessCastW64_25W256.get_cast st (at + 3)) `^` t3));
     } else {
       
     }
@@ -5127,17 +4985,13 @@ module M = {
     i <- 0;
     while ((i < (32 * (_LEN %/ 32)))) {
       x0 <-
-      (get256_direct (WArray800.init256 (fun i_0 => st.[i_0]))
-      ((4 * i) + (0 * 32)));
+      (ArrayAccessCastW256_25W256.get_cast_direct st ((4 * i) + (0 * 32)));
       x1 <-
-      (get256_direct (WArray800.init256 (fun i_0 => st.[i_0]))
-      ((4 * i) + (1 * 32)));
+      (ArrayAccessCastW256_25W256.get_cast_direct st ((4 * i) + (1 * 32)));
       x2 <-
-      (get256_direct (WArray800.init256 (fun i_0 => st.[i_0]))
-      ((4 * i) + (2 * 32)));
+      (ArrayAccessCastW256_25W256.get_cast_direct st ((4 * i) + (2 * 32)));
       x3 <-
-      (get256_direct (WArray800.init256 (fun i_0 => st.[i_0]))
-      ((4 * i) + (3 * 32)));
+      (ArrayAccessCastW256_25W256.get_cast_direct st ((4 * i) + (3 * 32)));
       i <- (i + 32);
       (x0, x1, x2, x3) <@ __4u64x4_u256x4 (x0, x1, x2, x3);
       Glob.mem <- (storeW256 Glob.mem buf0 x0);
@@ -5151,20 +5005,16 @@ module M = {
     }
     while ((i < (8 * (_LEN %/ 8)))) {
       t0 <-
-      (get64_direct (WArray800.init256 (fun i_0 => st.[i_0]))
-      ((4 * i) + (0 * 8)));
+      (ArrayAccessCastW64_25W256.get_cast_direct st ((4 * i) + (0 * 8)));
       Glob.mem <- (storeW64 Glob.mem (buf0 + i) t0);
       t1 <-
-      (get64_direct (WArray800.init256 (fun i_0 => st.[i_0]))
-      ((4 * i) + (1 * 8)));
+      (ArrayAccessCastW64_25W256.get_cast_direct st ((4 * i) + (1 * 8)));
       Glob.mem <- (storeW64 Glob.mem (buf1 + i) t1);
       t2 <-
-      (get64_direct (WArray800.init256 (fun i_0 => st.[i_0]))
-      ((4 * i) + (2 * 8)));
+      (ArrayAccessCastW64_25W256.get_cast_direct st ((4 * i) + (2 * 8)));
       Glob.mem <- (storeW64 Glob.mem (buf2 + i) t2);
       t3 <-
-      (get64_direct (WArray800.init256 (fun i_0 => st.[i_0]))
-      ((4 * i) + (3 * 8)));
+      (ArrayAccessCastW64_25W256.get_cast_direct st ((4 * i) + (3 * 8)));
       Glob.mem <- (storeW64 Glob.mem (buf3 + i) t3);
       i <- (i + 8);
     }
@@ -5174,20 +5024,16 @@ module M = {
     buf3 <- (buf3 + i);
     if ((0 < (_LEN %% 8))) {
       t0 <-
-      (get64_direct (WArray800.init256 (fun i_0 => st.[i_0]))
-      ((4 * i) + (0 * 8)));
+      (ArrayAccessCastW64_25W256.get_cast_direct st ((4 * i) + (0 * 8)));
       (buf0,  _0) <@ __m_ilen_write_upto8 (buf0, (_LEN %% 8), t0);
       t1 <-
-      (get64_direct (WArray800.init256 (fun i_0 => st.[i_0]))
-      ((4 * i) + (1 * 8)));
+      (ArrayAccessCastW64_25W256.get_cast_direct st ((4 * i) + (1 * 8)));
       (buf1,  _1) <@ __m_ilen_write_upto8 (buf1, (_LEN %% 8), t1);
       t2 <-
-      (get64_direct (WArray800.init256 (fun i_0 => st.[i_0]))
-      ((4 * i) + (2 * 8)));
+      (ArrayAccessCastW64_25W256.get_cast_direct st ((4 * i) + (2 * 8)));
       (buf2,  _2) <@ __m_ilen_write_upto8 (buf2, (_LEN %% 8), t2);
       t3 <-
-      (get64_direct (WArray800.init256 (fun i_0 => st.[i_0]))
-      ((4 * i) + (3 * 8)));
+      (ArrayAccessCastW64_25W256.get_cast_direct st ((4 * i) + (3 * 8)));
       (buf3,  _3) <@ __m_ilen_write_upto8 (buf3, (_LEN %% 8), t3);
     } else {
       
@@ -5227,20 +5073,9 @@ module M = {
     var status:W64.t;
     var t:W64.t;
     kst <- witness;
-    kst <-
-    (Array25.init
-    (fun i => (get256 (WArray808.init64 (fun i => st.[i])) (0 + i))));
+    kst <- (SubArrayDirect25W256_101W64.get_sub st 0);
     kst <@ __state_init_avx2x4 (kst);
-    st <-
-    (Array101.init
-    (WArray808.get64
-    (WArray808.init8
-    (fun i => (if ((32 * 0) <= i < ((32 * 0) + 800)) then (WArray800.get8
-                                                          (WArray800.init256
-                                                          (fun i => kst.[i]))
-                                                          (i - (32 * 0))) else 
-              (WArray808.get8 (WArray808.init64 (fun i => st.[i])) i)))
-    )));
+    st <- (SubArrayDirect25W256_101W64.set_sub st 0 kst);
     status <- (zeroextu64 trailb);
     status <- (status `<<` (W8.of_int 8));
     r64 <- (W8.to_uint ((W8.of_int r64) - (W8.of_int 1)));
@@ -5295,12 +5130,8 @@ module M = {
     trailb <- (trailb `<<` (t8 `&` (W8.of_int 63)));
     t128 <- (VMOV_64 trailb);
     t256 <- (VPBROADCAST_4u64 (truncateu64 t128));
-    t256 <-
-    (t256 `^` (get256_direct (WArray808.init64 (fun i => st.[i])) at));
-    st <-
-    (Array101.init
-    (WArray808.get64
-    (WArray808.set256_direct (WArray808.init64 (fun i => st.[i])) at t256)));
+    t256 <- (t256 `^` (ArrayAccessCastW256_101W64.get_cast_direct st at));
+    st <- (ArrayAccessCastW256_101W64.set_cast_direct st at t256);
     rbit <- (W64.of_int 1);
     rbit <- (rbit `<<` (W8.of_int 63));
     r8 <- (r8 - 1);
@@ -5308,19 +5139,12 @@ module M = {
     r8 <- (r8 `<<` 5);
     t128 <- (VMOV_64 rbit);
     t256 <- (VPBROADCAST_4u64 (truncateu64 t128));
-    t256 <-
-    (t256 `^` (get256_direct (WArray808.init64 (fun i => st.[i])) r8));
+    t256 <- (t256 `^` (ArrayAccessCastW256_101W64.get_cast_direct st r8));
+    st <- (ArrayAccessCastW256_101W64.set_cast_direct st r8 t256);
     st <-
-    (Array101.init
-    (WArray808.get64
-    (WArray808.set256_direct (WArray808.init64 (fun i => st.[i])) r8 t256)));
-    st <-
-    (Array101.init
-    (WArray808.get64
-    (WArray808.set32_direct (WArray808.init64 (fun i => st.[i]))
-    ((4 * 8) * 25)
-    ((get32_direct (WArray808.init64 (fun i => st.[i])) ((4 * 8) * 25)) `&`
-    (W32.of_int 4278255360)))));
+    (ArrayAccessCastW32_101W64.set_cast_direct st ((4 * 8) * 25)
+    ((ArrayAccessCastW32_101W64.get_cast_direct st ((4 * 8) * 25)) `&`
+    (W32.of_int 4278255360)));
     return st;
   }
   proc ststatus_updstate_avx2x4 (status:W8.t Array3.t, st:W64.t Array101.t) : 
@@ -5334,7 +5158,7 @@ module M = {
     status.[0] <- (truncateu8 (W64.of_int r8));
     status.[1] <- (truncateu8 (W64.of_int at));
     status.[2] <-
-    (get8_direct (WArray808.init64 (fun i => st.[i])) ((8 * 25) + 2));
+    (ArrayAccessCastW8_101W64.get_cast_direct st ((8 * 25) + 2));
     return status;
   }
   proc init_updstate_avx2x4 (st:W64.t Array101.t, r64:int, trailb:W8.t) : 
