proof/amd64/extracted/ArrayAccessCastW256_101W64.ec
@@ -1,0 +1,10 @@
+from Jasmin require import JWord JWord_array.
+
+require import ArrayWords101W64.
+
+clone export ArrayAccessCast as ArrayAccessCastW256_101W64  with op sizeWS <- 32,
+                                                                 op sizeWB <- 8,
+                                                                 op sizeB <- 101,
+                                                                 theory WordS <- W256,
+                                                                 theory WordB <- W64,
+                                                                 theory ArrayWordsB <= ArrayWords101W64.
