proof/amd64/extracted/ArrayAccessCastW256_999W8.ec
@@ -1,0 +1,10 @@
+from Jasmin require import JWord JWord_array.
+
+require import ArrayWords999W8.
+
+clone export ArrayAccessCast as ArrayAccessCastW256_999W8  with op sizeWS <- 32,
+                                                                op sizeWB <- 1,
+                                                                op sizeB <- 999,
+                                                                theory WordS <- W256,
+                                                                theory WordB <- W8,
+                                                                theory ArrayWordsB <= ArrayWords999W8.
