proof/amd64/extracted/ArrayAccessCastW32_101W64.ec
@@ -1,0 +1,10 @@
+from Jasmin require import JWord JWord_array.
+
+require import ArrayWords101W64.
+
+clone export ArrayAccessCast as ArrayAccessCastW32_101W64  with op sizeWS <- 4,
+                                                                op sizeWB <- 8,
+                                                                op sizeB <- 101,
+                                                                theory WordS <- W32,
+                                                                theory WordB <- W64,
+                                                                theory ArrayWordsB <= ArrayWords101W64.
