proof/amd64/extracted/ArrayAccessCastW32_26W64.ec
@@ -1,0 +1,10 @@
+from Jasmin require import JWord JWord_array.
+
+require import ArrayWords26W64.
+
+clone export ArrayAccessCast as ArrayAccessCastW32_26W64  with op sizeWS <- 4,
+                                                               op sizeWB <- 8,
+                                                               op sizeB <- 26,
+                                                               theory WordS <- W32,
+                                                               theory WordB <- W64,
+                                                               theory ArrayWordsB <= ArrayWords26W64.
