proof/amd64/extracted/ArrayAccessCastW64_25W256.ec
@@ -1,0 +1,10 @@
+from Jasmin require import JWord JWord_array.
+
+require import ArrayWords25W256.
+
+clone export ArrayAccessCast as ArrayAccessCastW64_25W256  with op sizeWS <- 8,
+                                                                op sizeWB <- 32,
+                                                                op sizeB <- 25,
+                                                                theory WordS <- W64,
+                                                                theory WordB <- W256,
+                                                                theory ArrayWordsB <= ArrayWords25W256.
