proof/amd64/extracted/ArrayAccessCastW8_26W64.ec
@@ -1,0 +1,10 @@
+from Jasmin require import JWord JWord_array.
+
+require import ArrayWords26W64.
+
+clone export ArrayAccessCast as ArrayAccessCastW8_26W64  with op sizeWS <- 1,
+                                                              op sizeWB <- 8,
+                                                              op sizeB <- 26,
+                                                              theory WordS <- W8,
+                                                              theory WordB <- W64,
+                                                              theory ArrayWordsB <= ArrayWords26W64.
