proof/amd64/extracted/ArrayWords101W64.ec
@@ -1,0 +1,9 @@
+from Jasmin require import JWord JWord_array.
+
+require import Array101 WArray808.
+
+clone export ArrayWords as ArrayWords101W64  with op sizeW <- 8,
+                                                  op sizeA <- 101,
+                                                  theory Word <= W64,
+                                                  theory ArrayN <= Array101,
+                                                  theory WArrayN <= WArray808.
