proof/amd64/extracted/ArrayWords25W256.ec
@@ -1,0 +1,9 @@
+from Jasmin require import JWord JWord_array.
+
+require import Array25 WArray800.
+
+clone export ArrayWords as ArrayWords25W256  with op sizeW <- 32,
+                                                  op sizeA <- 25,
+                                                  theory Word <= W256,
+                                                  theory ArrayN <= Array25,
+                                                  theory WArrayN <= WArray800.
