proof/amd64/extracted/ArrayWords25W64.ec
@@ -1,0 +1,9 @@
+from Jasmin require import JWord JWord_array.
+
+require import Array25 WArray200.
+
+clone export ArrayWords as ArrayWords25W64  with op sizeW <- 8,
+                                                 op sizeA <- 25,
+                                                 theory Word <= W64,
+                                                 theory ArrayN <= Array25,
+                                                 theory WArrayN <= WArray200.
