proof/amd64/extracted/ArrayWords26W64.ec
@@ -1,0 +1,9 @@
+from Jasmin require import JWord JWord_array.
+
+require import Array26 WArray208.
+
+clone export ArrayWords as ArrayWords26W64  with op sizeW <- 8,
+                                                 op sizeA <- 26,
+                                                 theory Word <= W64,
+                                                 theory ArrayN <= Array26,
+                                                 theory WArrayN <= WArray208.
