proof/amd64/extracted/ArrayWords999W8.ec
@@ -1,0 +1,9 @@
+from Jasmin require import JWord JWord_array.
+
+require import Array999 WArray999.
+
+clone export ArrayWords as ArrayWords999W8  with op sizeW <- 1,
+                                                 op sizeA <- 999,
+                                                 theory Word <= W8,
+                                                 theory ArrayN <= Array999,
+                                                 theory WArrayN <= WArray999.
