proof/amd64/extracted/SubArray25_26.ec
@@ -1,0 +1,7 @@
+from Jasmin require import JArray.
+
+require import Array25 Array26.
+
+clone export SubArray as SubArray25_26  with op sizeS <- 25, op sizeB <- 26,
+                                             theory ArrayS <= Array25,
+                                             theory ArrayB <= Array26.
