proof/amd64/extracted/SubArrayDirect25W256_101W64.ec
@@ -1,0 +1,12 @@
+from Jasmin require import JWord JWord_array.
+
+require import ArrayWords25W256 ArrayWords101W64.
+
+clone export SubArrayCast as SubArrayDirect25W256_101W64  with op sizeWS <- 32,
+                                                               op sizeWB <- 8,
+                                                               op sizeS <- 25,
+                                                               op sizeB <- 101,
+                                                               theory WordS <- W256,
+                                                               theory WordB <- W64,
+                                                               theory ArrayWordsS <= ArrayWords25W256,
+                                                               theory ArrayWordsB <= ArrayWords101W64.
